src/spec/TLS13.Wire.Spec.fsti
@@ -131,6 +131,11 @@ val serialize_handshake_msg:
   msg:M.handshake_msg ->
   GTot B.bytes
 
+val lemma_serialize_server_hello_len:
+  sh:M.server_hello ->
+  Lemma (B.length (serialize_handshake (M.ServerHello sh)) == 90 /\
+         B.length (serialize_handshake_msg (M.ServerHello sh)) == 90)
+
 val serialize_server_certificate_verify_input:
   transcript_hash:B.bytes ->
   GTot B.bytes
